plf/Smallstep.v
@@ -293,5 +293,15 @@ Proof.
     now apply step_eval with y.
 Qed.
 
+Ltac solve_by_inverts n :=
+  match goal with | H : ?T |- _ =>
+  match type of T with Prop =>
+    solve [
+      inversion H;
+      match n with S (S (?n')) => subst; solve_by_inverts (S n') end ]
+  end end.
 
+
+Ltac solve_by_invert :=
+  solve_by_inverts 1.
 
